FreeST/test/Programs/examples/io.fst
@@ -1,6 +1,6 @@
 main : ()
 main =
-    -- use stdout print functions
+    -- | use stdout print functions
     printBool     True;
     printBoolLn   False;
     printChar     'a';
@@ -9,15 +9,25 @@ main =
     printIntLn    2;
     printString   "Hello, ";
     printStringLn "World!";
-    -- print to stdout manually
+    -- | print to stdout manually
     receive_ @OutStream stdout & hPutStringLn "------------------" & select Close; 
-    -- print to stderr using put functions
+    -- | print to stderr using put functions
     putString "Error: " stderr; putStringLn "everything is fine!" stderr;
-    -- get values from stdin
+    -- | get values from stdin
     -- case inputBool   of { JustBool   b -> printBoolLn   b, NothingBool   -> printStringLn "oooops"};
     -- case inputInt    of { JustInt    i -> printIntLn    i, NothingInt    -> printStringLn "oooops"};
     -- case inputChar   of { JustChar   c -> printCharLn   c, NothingChar   -> printStringLn "oooops"};
     -- case inputString of { JustString s -> printStringLn s, NothingString -> printStringLn "oooops"};
-    -- unit!
-    printStringLn "";
+    -- | write to file
+    case openWriteFile "teste.txt" of {
+        JustS ch -> 
+            match hFilePutStringLn "Hello, World!" ch with {
+                Ok ch -> printStringLn "Ok!"; select Close ch & sink @Skip,
+                Error ch -> printStringLn "Error!"
+            },
+        NothingS -> ()
+    };
+    -- | extra print
+    printStringLn "-end-";
+    -- | unit!
     ()
